---
title: "ARMA models II"
subtitle: "Lecture 10"
format: revealjs
auto-stretch: false
filters:
  - shinylive
---

## Where were we?

$$
y_t
=
\beta_0
+
\underbrace{\sum\limits_{l=1}^p\beta_ly_{t-l}}_{\text{autoregressive}}
+
\underbrace{\sum_{i=1}^q\theta_i\varepsilon_{t-i}}_{\text{moving average}}
+
\varepsilon_t,
\quad
\varepsilon_t
\iid
\N(0\com \sigma^2)
.
$$

. . .

Can't do anything analytically:

::: incremental 
- MLE requires numerical optimization;
- Bayes requires ugly MCMC;
- Forecasts with correct uncertainty quantification are hard;
- Bootstrapping is a pain;
- Model combination is probably not worth it.
:::

## The bottom line, at the top 

::: incremental 
- A stationary AR(p) can be written as an MA$(\infty)$;
- An "invertible" MA(q) can be written as an AR$(\infty)$;
- A stationary and invertible ARMA(p, q) can be written as either an MA$(\infty)$ or an AR$(\infty)$.
:::

. . .

These suggest *approximations* that can ease the computational burden of estimation and forecasting.

# Quick background

## Lag operator

::: callout-note
## Definition
The **lab operator** $L$ acts on a time series $y_t$ to return its first lagged value:

$$
Ly_{t}=y_{t-1}.
$$
:::

. . .

Imagine multiple applications:

$$
L^2 y_{t}= L L y_{t}=L y_{t-1}=y_{t-2}.
$$

. . .

In general: 

$$
L^ky_t=y_{t-k}.
$$

## AR(1)

$$
\begin{aligned}
y_t
&=
\beta_1y_{t-1}+\varepsilon_t
\\
y_t
&=
\beta_1 Ly_t+\varepsilon_t
\\
y_t
-
\beta_1 Ly_t
&=
\varepsilon_t
\\
(1
-
\beta_1 L)y_t
&=
\varepsilon_t.
\end{aligned}
$$

## AR(2)

$$
\begin{aligned}
y_t
&=
\beta_1y_{t-1}+\beta_2y_{t-2}+\varepsilon_t
\\
y_t
&=
\beta_1Ly_t+\beta_2L^2y_t+\varepsilon_t
\\
y_t
-
\beta_1Ly_t-\beta_2L^2y_t
&=
\varepsilon_t
\\
(1
-
\beta_1 L-\beta_2L^2)y_t
&=
\varepsilon_t.
\end{aligned}
$$

## The AR(p)

Old way of writing it:

$$
y_t=\sum\limits_{l=1}^p\beta_ly_{t-l}+\varepsilon_t.
$$

. . .

New way of writing it:

$$
\left(1-\sum\limits_{l=1}^p\beta_lL^l\right)y_t=\varepsilon_t.
$$

## The AR polynomial

::: callout-tip
## Definition
If $\beta_{1:p}$ are the non-zero coefficients of an AR(p), then the **AR polynomial** is 

$$
\beta(z) = 1-\beta_1z-\beta_2z^2-...-\beta_pz^p,\quad z\in\mathbb{C}.
$$
:::

. . .

Plug in the lag operator $L$, and we see that the AR(p) is

$$
\beta(L)y_t=\varepsilon_t.
$$

## MA(1)

$$
\begin{aligned}
y_t
&=
\varepsilon_t+\theta_1\varepsilon_{t-1}
\\
&=
\varepsilon_t+\theta_1L\varepsilon_t
\\
&=
(1+\theta_1L)\varepsilon_t.
\\
\end{aligned}
$$

## MA(2)

$$
\begin{aligned}
y_t
&=
\varepsilon_t+\theta_1\varepsilon_{t-1} + \theta_2\varepsilon_{t-2}
\\
&=
\varepsilon_t+\theta_1L\varepsilon_t + \theta_2L^2\varepsilon_{t}
\\
&=
(1+\theta_1L+\theta_2L^2)\varepsilon_t.
\\
\end{aligned}
$$

## The MA(q)

Old way of writing it:

$$
y_t
=
\sum_{i=1}^q\theta_i\varepsilon_{t-i}
+
\varepsilon_t.
.
$$

. . .

New way of writing it:

$$
y_t=\left(1+\sum\limits_{i=1}^q\theta_iL^i\right)\varepsilon_t.
$$

## The MA polynomial


::: callout-tip
## Definition
If $\theta_{1:q}$ are the non-zero coefficients of an MA(q), then the **MA polynomial** is 

$$
\theta(z) = 1+\theta_1z+\theta_2z^2+...+\theta_qz^q,\quad z\in\mathbb{C}.
$$
:::

. . .

Plug in the lag operator $L$, and we see that the MA(q) is

$$
y_t=\theta(L)\varepsilon_t.
$$

## ARMA(1, 1)

$$
\begin{aligned}
y_t
&=
\beta_1y_{t-1}
+
\varepsilon_t+\theta_1\varepsilon_{t-1}
\\
y_t
&=
\beta_1Ly_t
+
(1+\theta_1L)\varepsilon_t
\\
(1-\beta_1L)
y_t
&=
(1+\theta_1L)\varepsilon_t.
\end{aligned}
$$

## ARMA(p, q)

Old way of writing it:

$$
y_t
=
\sum\limits_{l=1}^p\beta_ly_{t-l}
+
\sum_{i=1}^q\theta_i\varepsilon_{t-i}
+
\varepsilon_t
$$

. . .

New way of writing it:

$$
\begin{aligned}
\beta(L)y_t
&=
\theta(L)\varepsilon_t.
\end{aligned}
$$

## A tale of two polynomials

The ARMA(p, q):

$$
\beta(L)y_t
=
\theta(L)\varepsilon_t,
\quad\varepsilon\iid\N(0\com\sigma^2).
$$

. . .

Much hinges on the properties of these two goofy polynomials of a complex argument:

$$
\begin{aligned}
\beta(z)&=1-\sum\limits_{l=1}^p\beta_lz^l\\
\theta(z)&=1+\sum\limits_{i=1}^q\theta_iz^i.
\end{aligned}
$$

## Question

. . .


Can we write this?

$$
y_t=\frac{\theta(L)}{\beta(L)}\varepsilon_t.
$$

. . .

Can we write this?

$$
\frac{\beta(L)}{\theta(L)}y_t=\varepsilon_t.
$$

. . .

The *inverses* $1/\beta(L)$ and $1/\theta(L)$ only converge if the respective polynomials have roots *outside* the unit circle. Are you tingling?

# Rewrite AR(p) as MA($\infty$)

## Example: AR(1) as MA($\infty$)

Assuming mean-zero ($\beta_0=0$), we know

$$
\begin{aligned}
y_1&=\beta_1y_0+\varepsilon_1\\
y_2&=\beta_1y_1+\varepsilon_2\\
y_3&=\beta_1y_2+\varepsilon_3\\
&\vdots\\
y_{t-1}&=\beta_1y_{t-2}+\varepsilon_{t-1}\\
y_t&=\beta_1y_{t-1}+\varepsilon_t\\
&\vdots
\end{aligned}
$$

## Example: AR(1) as MA($\infty$)

Apply recursive substitution:

$$
\begin{aligned}
y_t
&=
\beta_1y_{t-1}+\varepsilon_t\\
&=
\beta_1(\beta_1y_{t-2}+\varepsilon_{t-1})+\varepsilon_t\\
&=
\beta_1^2y_{t-2}+\beta_1\varepsilon_{t-1}+\varepsilon_t\\
&=
\beta_1^2(\beta_1y_{t-3}+\varepsilon_{t-2})+\beta_1\varepsilon_{t-1}+\varepsilon_t\\
&=
\beta_1^3y_{t-3}+\beta_1^2\varepsilon_{t-2}+\beta_1\varepsilon_{t-1}+\varepsilon_t\\
&\vdots\\
&=
\beta_1^ky_{t-k}
+
\sum\limits_{j=0}^{k-1}\beta_1^j\varepsilon_{t-j}
\\
&\vdots
\end{aligned}
$$

## Example: AR(1) as MA($\infty$)

Keep doing that forever, and eventually

$$
y_t
=
\sum\limits_{j=0}^\infty \beta_1^j\varepsilon_{t-j}.
$$
In order for the right-hand side to be finite, we need $|\beta_1|<1$. 

In other words, the AR(1) has to be stationary.

## In general: AR(p) as MA($\infty$)

::: callout-tip
## MA($\infty$) representation
If an AR(p) is stationary, then it can be written

$$
y_t=\frac{1}{\beta(L)}\varepsilon_t=\sum\limits_{j=0}^\infty \psi_j\varepsilon_{t-j},
$$
where $\psi_0=1$ and $\sum_{j=0}^\infty |\psi_j|<\infty$.

:::

. . .

In other words, there is an infinite order MA polynomial

$$
\psi(z)=1+\psi_1z+\psi_2z^2+\psi_3z^3+...
$$

and $y_t=\psi(L)\varepsilon_t$.

## Stationarity redux {.medium}

Companion form matrix:

$$
\BG
=
\begin{bmatrix}
\beta_1 & \beta_2  & \cdots & \beta_{p-1} & \beta_p\\
1 & 0  & \cdots & 0 & 0\\
0 & 1  & \cdots & 0 & 0\\
\vdots & \vdots  & \ddots & \vdots & \vdots\\
0 & 0  & \cdots & 1 & 0
\end{bmatrix}
$$

. . .

AR polynomial:

$$
\beta(z) = 1-\beta_1z-\beta_2z^2-...-\beta_pz^p
$$

. . .

$\BG$ having eigenvalues *inside* the unit circle is the same as $\beta(z)$ having roots *outside* the unit circle.

## Eigenvalues of the companion matrix

The eigenvalues solve 

$$
\det(\BG-\lambda\BI_p)=0
$$

. . .

If $p=2$, 

$$
\begin{aligned}
\det\begin{pmatrix}
\beta_1-\lambda & \beta_2\\
1 & -\lambda
\end{pmatrix}
&=
-\lambda(\beta_1-\lambda)-\beta_2
\\
&=
\lambda^2-\beta_1\lambda-\beta_2.
\end{aligned}
$$

. . .

In general, you can show that

$$
\det(\BG-\lambda\BI_p)
=
\lambda^p
-
\beta_1\lambda^{p-1}
-
\beta_2\lambda^{p-2}
-
\cdots 
-
\beta_p
.
$$

## Relation to the AR polynomial

Eigenvalues of $\BG$ are roots of: 

$$
g(\lambda)=
\lambda^p
-
\beta_1\lambda^{p-1}
-
\beta_2\lambda^{p-2}
-
\cdots 
-
\beta_p.
$$

. . .

Notice that 

$$
\begin{aligned}
\beta(1/\lambda) &= 1-\frac{\beta_1}{\lambda}-\frac{\beta_2}{\lambda^2}-...-\frac{\beta_p}{\lambda^p}
\\
&=
\frac{\lambda^p}{\lambda^p}
\left(
1-\frac{\beta_1}{\lambda}-\frac{\beta_2}{\lambda^2}-...-\frac{\beta_p}{\lambda^p}\right)\\
&=
\frac{1}{\lambda^p}(\lambda^p
-
\beta_1\lambda^{p-1}
-
\beta_2\lambda^{p-2}
-
\cdots 
-
\beta_p)
\\
&=
g(\lambda)/\lambda^p.
\end{aligned}
$$

## Main idea

. . .

- We know 

$$
\beta\left(\frac{1}{\lambda}\right)=\frac{g(\lambda)}{\lambda^{p}}.
$$

. . .

- The roots of $\beta(z)$ and the roots of $g(\lambda)$ are reciprocals of one another;

. . .

- If $|\lambda|<1$, then $|1/\lambda|=1/|\lambda|>1$. 

## Where do the new coefficients come from?

Theoretically, we have 

$$
y_t=\frac{1}{\beta(L)}\varepsilon_t=\psi(L)\varepsilon_t,
$$

so whatever they are, the $\psi_j$ solve

$$
\psi(z)=\sum\limits_{j=0}^\infty\psi_jz^j=\frac{1}{\beta(z)}=\frac{1}{1-\sum\limits_{l=1}^p\beta_lz^l}.
$$

## Parting thought: summability

- The assumptions of the theorem (stationary AR) are enough to guarantee absolute summability;
- The MA($\infty$) would remain coherent if we only had square summability, but it wouldn't be *ergodic*.

## Ergodicity {.medium}

::: callout-note
## Law of large numbers for dependent sequences
If $y_t$ is stationary with $E(y_t) = \mu$, $\gamma(h)=\cov(y_{t+h},\,y_t)$, and

$$
\sum\limits_{h=0}^\infty|\gamma(h)|<\infty,
$$

then 

$$
\bar{y}_T=\frac{1}{T}\sum\limits_{t=1}^Ty_t\overset{L^2}{\to}\mu.
$$

Which implies convergence in probability, distribution, etc.

:::

::: incremental 
- This is what is meant by *ergodic*;
- Without it, stuff like method-of-moments breaks down;
- Square summable is not enough.
:::

# Rewrite MA(q) as AR$(\infty)$


## Example: MA(1) as AR$(\infty)$

We know that 

$$
\begin{aligned}
y_1&=\varepsilon_1+\theta_1\varepsilon_{0} &&\implies &&\varepsilon_1=y_1-\theta_1\varepsilon_0\\
y_2&=\varepsilon_2+\theta_1\varepsilon_{1} &&\implies &&\varepsilon_2=y_2-\theta_1\varepsilon_1\\
y_3&=\varepsilon_3+\theta_1\varepsilon_{2} &&\implies &&\varepsilon_3=y_3-\theta_1\varepsilon_2\\
& &&\vdots\\
y_{t-1}&=\varepsilon_{t-1}+\theta_1\varepsilon_{t-2} &&\implies &&\varepsilon_{t-1}=y_{t-1}-\theta_1\varepsilon_{t-2}\\
y_t&=\varepsilon_t+\theta_1\varepsilon_{t-1} &&\implies &&\varepsilon_t=y_t-\theta_1\varepsilon_{t-1}\\
& &&\vdots
\end{aligned}
$$

## Example: MA(1) as AR$(\infty)$

Recursive substitution:

$$
\begin{aligned}
\varepsilon_t
&=
y_t
-
\theta_1\varepsilon_{t-1}
\\
&=
y_t
-
\theta_1(y_{t-1}-\theta_1\varepsilon_{t-2})
\\
&=
y_t
-
\theta_1y_{t-1}+\theta_1^2\varepsilon_{t-2}
\\
&=
y_t
-
\theta_1y_{t-1}+\theta_1^2(y_{t-2}-\theta_1\varepsilon_{t-3})
\\
&=
y_t
-
\theta_1y_{t-1}+\theta_1^2y_{t-2}-\theta_1^3\varepsilon_{t-3}
\\
&\vdots \\
&=
\sum\limits_{j=0}^{k-1} (-\theta_1)^jy_{t-j} + (-\theta_1)^{k}\varepsilon_{t-k}
\\
&\vdots 
\end{aligned}
$$

## Example: MA(1) as AR$(\infty)$

Keep doing that forever, and eventually

$$
\varepsilon_t
=
\sum\limits_{j=0}^\infty (-\theta_1)^jy_{t-j}.
$$
In order for the right-hand side to be finite, we need $|\theta_1|<1$. 

In other words, the MA(1) has to be identified.

## Invertibility

If the MA polynomial 

$$
\theta(z)=1+\theta_1z+\theta_2z^2+...+\theta_qz^q
$$

has roots outside the unit circle, then we can *invert*:

$$
y_t=\theta(L)\varepsilon_t\quad \Longleftrightarrow\quad \frac{1}{\theta(L)}y_t=\varepsilon_t
$$

This condition on the roots is also what ensures *identification*.

## In general: MA(q) as AR$(\infty)$

::: callout-tip
## AR($\infty$) representation
If an MA(q) is invertible, then it can be written

$$
\varepsilon_t=\frac{1}{\theta(L)}y_t=\sum\limits_{j=0}^\infty \pi_jy_{t-j},
$$
where $\pi_0=1$ and $\sum_{j=0}^\infty |\pi_j|<\infty$.

:::

. . .

In other words, there is an infinite order AR polynomial

$$
\pi(z)=1+\pi_1z+\pi_2z^2+\pi_3z^3+...
$$

and $\varepsilon_t=\pi(L)y_t$.

## Where do the new coefficients come from?

Theoretically, we have 

$$
\varepsilon_t=\frac{1}{\theta(L)}y_t=\pi(L)y_t,
$$

so whatever they are, the $\pi_j$ solve

$$
\pi(z)=\sum\limits_{j=0}^\infty\pi_jz^j=\frac{1}{\theta(z)}=\frac{1}{1+\sum\limits_{i=1}^q\theta_iz^i}.
$$

# Rewrite ARMA as pure AR or MA

## Putting it together {.medium}

We know:

$$
\beta(L)y_t
=
\theta(L)\varepsilon_t.
$$

. . .

If it's stationary, you get an MA($\infty$):

$$
y_t=\frac{\theta(L)}{\beta(L)}\varepsilon_t.
$$

. . .

If it's invertible, you get an AR($\infty$):

$$
\frac{\beta(L)}{\theta(L)}y_t=\varepsilon_t.
$$


. . .

If it's both stationary and invertible, take your pick.


## ARMA as MA($\infty$)

A stationary ARMA(p, q) can be written

$$
y_t=\sum\limits_{j=0}^\infty \psi_j\varepsilon_{t-j},
$$

where the $\psi_j$ solve 

$$
\psi(z)=\sum\limits_{j=0}^\infty \psi_jz^j=\frac{\theta(z)}{\beta(z)},\quad |z|\leq 1.
$$

How?

## Recursion for the new weights {.small}

Match the coefficients:

$$
\begin{aligned}
\psi(z)
&=\frac{\theta(z)}{\beta(z)}
\\
\beta(z)\psi(z)
&=\theta(z)
\\
(1-\beta_1z-\beta_2z^2-...-\beta_pz^p)(1+\psi_1z+\psi_2z^2+...)
&=
1+\theta_1z+\theta_2z^2+...+\theta_qz^q.
\end{aligned}
$$

. . .

Multiply the left side out, and it must be that 

$$
\begin{aligned}
\psi_0 &= 1, \\
\psi_1 - \beta_1 \psi_0 &= \theta_1, \\
\psi_2 - \beta_1 \psi_1 - \phi_2 \psi_0 &= \theta_2, \\
\psi_3 - \beta_1 \psi_2 - \phi_2 \psi_1 - \phi_3 \psi_0 &= \theta_3, \\
&\ \ \vdots
\end{aligned}
$$

## In general

Get a computer to grind through:

$$
\psi_j - \sum_{k=1}^p \beta_k \psi_{j-k} = 0, 
\qquad j \geq \max(p, q+1)
$$

and 

$$
\psi_j - \sum_{k=1}^j \beta_k \psi_{j-k} = \theta_j, 
\qquad 0 \leq j < \max(p, q+1).
$$


## ARMA as AR($\infty$)

A invertible ARMA(p, q) can be written

$$
\varepsilon_t=\sum\limits_{j=0}^\infty \pi_jy_{t-j},
$$

where the $\pi_j$ solve 

$$
\pi(z)=\sum\limits_{j=0}^\infty \pi_jz^j=\frac{\beta(z)}{\theta(z)},\quad |z|\leq 1.
$$

Weights follow similar idea from before. Just let a computer do it.

## Big ol' theorem {.small}

::: callout-important
## Wold representation

Any stationary mean-zero process $y_t$ can be uniquely written as 

$$
y_t=\nu_t+\sum\limits_{j=0}^\infty \psi_j\varepsilon_{t-j},
$$

where 

- $\varepsilon_t$ uncorrelated with variance $\sigma^2>0$;
- $\psi_j$ square summable;
- $\nu_t$ perfectly predictable given its history (*deterministic*).

:::

. . .

Shumway and Stoffer:

> The theorem...falls short of our needs because we would prefer the noise process...to be independent...$\{\psi_j\}$ to be absolutely summable. But the decomposition does give us the confidence that we will not be completely oï¬€ the mark by fitting ARMA models to many types of time series.

. . .

Whatever.